theories/ftlr/Mov.v
@@ -4,7 +4,7 @@ From iris.program_logic Require Import weakestpre adequacy lifting.
 From stdpp Require Import base.
 From cap_machine.ftlr Require Import ftlr_base.
 From cap_machine.rules Require Import rules_base rules_Mov.
-From cap_machine.proofmode Require Import map_simpl.
+From cap_machine.proofmode Require Import map_simpl register_tactics.
 From cap_machine Require Import stdpp_extra.
 
 Section fundamental.
@@ -27,16 +27,16 @@ Section fundamental.
   Implicit Types w : (leibnizO Word).
   Implicit Types interp : (D).
 
-   Lemma mov_case (W : WORLD) (regs : leibnizO Reg) (p : Perm)
-        (g : Locality) (b e a : Addr) (w : Word) (ρ : region_type) (dst : RegName) (src : Z + RegName) (P:D):
-    ftlr_instr W regs p g b e a w (Mov dst src) ρ P.
+   Lemma mov_case (W : WORLD) (regs : leibnizO Reg)
+     (p p' : Perm) (g : Locality) (b e a : Addr)
+     (w : Word) (ρ : region_type) (dst : RegName) (src : Z + RegName) (P:D):
+    ftlr_instr W regs p p' g b e a w (Mov dst src) ρ P.
   Proof.
-    intros Hp Hsome i Hbae Hpers Hpwl Hregion Hnotrevoked Hnotmonostatic Hi.
-    iIntros "#IH #Hinv_interp #Hreg #Hinva #Hrcond #Hwcond Hmono Hw Hsts Hown".
+    intros Hp Hsome i Hbae Hfp HO Hpers Hpwl Hregion Hnotrevoked Hnotfrozen Hi.
+    iIntros "#IH #Hinv_interp #Hreg #Hinva #Hrcond #Hwcond #Hmono Hw Hsts Hown".
     iIntros "Hr Hstate Ha HPC Hmap".
     iDestruct (execCond_implies_region_conditions with "Hinv_interp") as "#Hinv"; eauto.
-    iDestruct ((big_sepM_delete _ _ PC) with "[HPC Hmap]") as "Hmap /=";
-      [apply lookup_insert|rewrite delete_insert_delete;iFrame|]. simpl.
+    iInsert "Hmap" PC.
     iApply (wp_Mov with "[$Ha $Hmap]"); eauto.
     { simplify_map_eq; auto. }
     { rewrite /subseteq /map_subseteq. intros rr _.
@@ -47,45 +47,46 @@ Section fundamental.
     - iApply wp_pure_step_later; auto. iNext; iIntros "_".
       iApply wp_value; auto. iIntros; discriminate.
     - incrementPC_inv; simplify_map_eq.
-      rename x into p'
-      ; rename x0 into g'
-      ; rename x1 into b'
-      ; rename x2 into e'
-      ; rename x3 into a'
-      ; rename x4 into a''.
+      rename x into p0
+      ; rename x0 into g0
+      ; rename x1 into b0
+      ; rename x2 into e0
+      ; rename x3 into a0
+      ; rename x4 into a0'.
       iApply wp_pure_step_later; auto; iNext; iIntros "_".
 
       destruct (decide (dst = PC)) as [HdstPC|HdstPC]; simplify_map_eq.
       { map_simpl "Hmap".
         destruct src; simpl in *; try discriminate.
         iDestruct (region_close with "[$Hstate $Hr $Ha $Hmono Hw]") as "Hr"; eauto.
-        { destruct ρ;auto;[|specialize (Hnotmonostatic g0)];contradiction. }
+        { destruct ρ;auto;[|ospecialize (Hnotfrozen _)];contradiction. }
         destruct (decide (r = PC)).
         + simplify_map_eq.
           iApply ("IH" $! _ regs with "[%] [] [Hmap] [$Hr] [$Hsts] [$Hown]"); try iClear "IH"; eauto.
           rewrite !fixpoint_interp1_eq /=.
           destruct Hp as [-> | [  -> | [-> ->] ] ]; rewrite /region_conditions //=.
         + simplify_map_eq.
-          iDestruct ("Hreg" $! r (WCap p' g' b' e' a') n H ) as "Hr0".
-          destruct (PermFlowsTo RX p') eqn:Hpft.
+          iDestruct ("Hreg" $! r (WCap p0 g0 b0 e0 a0) n H ) as "Hr0".
+          destruct (PermFlowsTo RX p0) eqn:Hpft.
         - iApply ("IH" $! _ regs with "[%] [] [Hmap] [$Hr] [$Hsts] [$Hown]"); try iClear "IH"; eauto.
-          { destruct p'; simpl in Hpft; auto.
+          { destruct p0; simpl in Hpft; auto.
             repeat rewrite fixpoint_interp1_eq; simpl.
-            destruct g'; auto.
+            destruct g0; auto.
           }
           { rewrite !fixpoint_interp1_eq /=.
-            destruct p',g'; try congruence; rewrite /region_conditions //=.
+            destruct p0,g0; try congruence; rewrite /region_conditions //=.
           }
         - iApply (wp_bind (fill [SeqCtx])).
-          iDestruct ((big_sepM_delete _ _ PC) with "Hmap") as "[HPC Hmap]"; [apply lookup_insert|].
-          iApply (wp_notCorrectPC with "HPC"); [eapply not_isCorrectPC_perm; destruct p'; simpl in Hpft; try discriminate; eauto|].
+          iExtract "Hmap" PC as "HPC".
+          iApply (wp_notCorrectPC with "HPC")
+          ; first (eapply not_isCorrectPC_perm; destruct p0; simpl in Hpft; try discriminate; eauto).
           iNext. iIntros "HPC /=".
           iApply wp_pure_step_later; auto;iNext; iIntros "_".
           iApply wp_value.
           iIntros. discriminate. }
       { map_simpl "Hmap".
         iDestruct (region_close with "[$Hstate $Hr $Ha $Hmono Hw]") as "Hr"; eauto.
-        { destruct ρ;auto;[|specialize (Hnotmonostatic g)];contradiction. }
+        { destruct ρ;auto;[|ospecialize (Hnotfrozen _)];contradiction. }
         iApply ("IH" $! _ (<[dst:=w0]> _) with "[%] [] [Hmap] [$Hr] [$Hsts] [$Hown]"); eauto.
         - intros; simpl.
           rewrite lookup_insert_is_Some.
@@ -96,14 +97,15 @@ Section fundamental.
             destruct src; simplify_map_eq.
             * repeat rewrite fixpoint_interp1_eq; auto.
             * destruct (decide (PC = r)); simplify_map_eq.
-              ** rewrite (fixpoint_interp1_eq _ (WCap p' g' b' e' a')) /=.
-                 destruct Hp as [Hp | [Hp | [Hp Hg] ] ]; subst p'; try subst g';
+              ** rewrite (fixpoint_interp1_eq _ (WCap p0 g0 b0 e0 a0)) /=.
+                 destruct Hp as [Hp | [Hp | [Hp Hg] ] ]; subst p0; try subst g0;
                    try (iFrame "Hexec"); try (iFrame "Hinv").
                  all: iApply (big_sepL_mono with "Hinv").
-                 all: intros; iIntros "(H & ?)".
-                 all: simpl; try (iDestruct "H" as (P') "(?&?&?)").
-                 iExists _; iFrame.
-                 iExists RWLX; iFrame; iPureIntro ; done.
+                 all: intros; iIntros "H".
+                 all: simpl.
+                 all: iDestruct "H" as (p Hfl) "[H %Hstate]".
+                 1: iDestruct "H" as (P' HpersP') "H".
+                 all: iExists p; iFrame "%∗".
               ** iApply ("Hreg" $! r) ; auto.
           }
           { iApply ("Hreg" $! ri) ; auto. }
